LocalReasoning.v
@@ -1,79 +1,45 @@
-From Celsius Require Export Trees.
-From Celsius Require Export Eval.
-From Celsius Require Export PartialMonotonicity.
-From Celsius Require Export Reachability.
-From Celsius Require Export Compatibility.
-From Celsius Require Export Scopability.
-From Celsius Require Export Stackability.
-From Celsius Require Export Wellformedness.
-Require Import ssreflect ssrbool.
-Require Import Psatz.
-
-Require Import Sets.Ensembles.
-Require Import List.
+From Celsius Require Export Trees Eval PartialMonotonicity Reachability Compatibility Scopability Stackability Wellformedness.
+Require Import ssreflect ssrbool Psatz Sets.Ensembles List.
 Import ListNotations.
 Open Scope nat_scope.
 
 
-Module LocalReasoning.
-  Import Eval.Evaluator.
-  Import Reachability.Reachability.
-  Import Scopability.Scopability.
-  Import Compatibility.Compatibility.
-  Import PartialMonotonicity.PartialMonotonicity.
-  Import Stackability.Stackability.
-  Import Wellformedness.Wellformedness.
 
-  Lemma local_reasoning:
-    forall σ σ' L L',
-      L ⪽ σ ->
-      L' ⪽ σ' ->
-      (σ, L) ⋖ (σ', L') ->
-      σ ≪ σ' ->
-      σ ⊆ σ' ->
-      σ ⪯ σ' ->
-      (σ ⊫ L : hot) ->
-      σ' ⊫ L' : hot.
-  Proof.
-    intros σ σ' L L' H H0 H1 H2 H3 H4 H5.
-    intros l0 Hl0. unfold reachable_hot. intros l1 Hl1.
-    move : (partialMonotonicity_domains _ _ H4) => H_dom.
-    destruct (PeanoNat.Nat.lt_ge_cases l1 (dom σ)).
-    + (* l ∈ (dom σ) *)
-      assert (reachability_set σ L l1). {
-        apply H1; simpl => //.
-        exists l0 => //.
-      }
-      move : H7 => [l2 [Hl2_dom Hl2_rch]].
-      move : (H5 l2 Hl2_dom l1 Hl2_rch).
-      eapply partialMonotonicity_warm_monotone; eauto.
-    +
-      unfold stackability in H2.
-      move /(_ l1):H2 => H2.
-      pose proof (proj2 (reachability_dom _ _ _ Hl1)). intuition.
-  Qed.
+Lemma local_reasoning:
+  forall σ σ' L L',
+    L ⪽ σ ->
+    L' ⪽ σ' ->
+    (σ, L) ⋖ (σ', L') ->
+    σ ≪ σ' ->
+    σ ⊆ σ' ->
+    σ ⪯ σ' ->
+    (σ ⊫ L : hot) ->
+    σ' ⊫ L' : hot.
+Proof.
+  intros; intros l' Hl'.
+  assert (dom σ <= dom σ') by eauto with pM.
+  destruct (PeanoNat.Nat.lt_ge_cases l' (dom σ)).
+  + (* l ∈ (dom σ) *)
+    eapply partialMonotonicity_warm_monotone; eauto .
+    assert (reachability_set σ L l'). by (eapply H1; simpl => //; eexists; eauto).
+    inversion H9; steps.
+    eapply H5; eauto with rch.
+  + eapply reachability_dom, H2 in Hl'; intuition.
+Qed.
 
 
-  Theorem Local_reasoning:
-    forall e σ σ' ρ ψ l k,
-      ⟦e⟧(σ, ρ, ψ)(k) = (Success l σ') ->
-      wf σ -> (codom ρ ∪ {ψ}) ⪽ σ ->
-      (σ ⊫ ((codom ρ) ∪ {ψ}) : hot) ->
-      σ' ⊨ l : hot.
-  Proof.
-    intros.
-    assert (σ' ⊫ (Singleton Loc l) : hot). {
-      eapply local_reasoning;
-        eauto using stackability_theorem, compatibility_theorem, partialMonotonicity_theorem.
-
-      pose proof (wellformedness_conserved _ _ _ _ _ _ _ H H0 H1) as [A1 A2].
-      unfold storeSubset; intros. induction H3 => //.
-      pose proof (scopability_theorem _ _ _ _ _ _ _ H) as [A2 A3] => //.
-    }
-      by apply (H3 l).
-  Qed.
-
-  Print DependGraph Local_reasoning.
-
-
-  End LocalReasoning.
+Theorem Local_reasoning:
+  forall e σ σ' ρ ψ l k,
+    ⟦e⟧(σ, ρ, ψ)(k) = (Success l σ') ->
+    wf σ ->
+    (codom ρ ∪ {ψ}) ⪽ σ ->
+    (σ ⊫ ((codom ρ) ∪ {ψ}) : hot) ->
+    σ' ⊨ l : hot.
+Proof.
+  intros.
+  assert (σ' ⊫ (Singleton Loc l) : hot). {
+    eapply local_reasoning;
+      eauto using stackability_theorem with pM stk cmpt wf lia.
+    eapply scopability_theorem in H; eauto with pM wf lia; steps. }
+  eapply H3; eauto using In_singleton.
+Qed.
